theories/lang_generic_sem.v
@@ -1,0 +1,183 @@
+From gitrees Require Import prelude.
+From gitrees Require Import gitree.
+Require Import List.
+Import ListNotations.
+
+Section interp.
+  Local Open Scope type.
+  Context {E: opsInterp}.
+  Context {R} `{!Cofe R}.
+  Notation IT := (IT E R).
+  Notation ITV := (ITV E R).
+
+  Fixpoint interp_scope (S : scope) : ofe :=
+    match S with
+    | [] => unitO
+    | τ::Sc => prodO IT (interp_scope Sc)
+    end.
+
+  Instance interp_scope_cofe S : Cofe (interp_scope S).
+  Proof. induction S; simpl; apply _. Qed.
+
+  Instance interp_scope_inhab S : Inhabited (interp_scope S).
+  Proof. induction S; simpl; apply _. Defined.
+
+  Equations interp_var {S : scope} (v : var S) : interp_scope S -n> IT :=
+    interp_var (S:=(_::_))     Vz := fstO;
+    interp_var (S:=(_::Sc)) (Vs v) := interp_var v ◎ sndO.
+
+  Instance interp_var_ne S (v : var S) : NonExpansive (@interp_var S v).
+  Proof.
+    intros n D1 D2 HD12. induction v; simp interp_var.
+    - by f_equiv.
+    - eapply IHv. by f_equiv.
+  Qed.
+
+  Global Instance interp_var_proper S (v : var S) : Proper ((≡) ==> (≡)) (interp_var v).
+  Proof. apply ne_proper. apply _. Qed.
+
+  Definition interp_scope_split {S1 S2} :
+    interp_scope (S1 ++ S2) -n> interp_scope S1 * interp_scope S2.
+  Proof.
+    induction S1 as [|? S1]; simpl.
+    - simple refine (λne x, (tt, x)).
+      solve_proper.
+    - simple refine (λne xy, let ss := IHS1 xy.2 in ((xy.1, ss.1), ss.2)).
+      solve_proper.
+  Defined.
+
+  (** scope substituions *)
+  Inductive ssubst : scope → Type :=
+  | emp_ssubst : ssubst []
+  | cons_ssubst {S} : ITV → ssubst S → ssubst (tt::S)
+  .
+
+  Equations interp_ssubst {S} (ss : ssubst S) : interp_scope S :=
+    interp_ssubst emp_ssubst := tt;
+    interp_ssubst (cons_ssubst αv ss) := (IT_of_V αv, interp_ssubst ss).
+
+  Equations list_of_ssubst {S} (ss : ssubst S) : list ITV :=
+    list_of_ssubst emp_ssubst := [];
+    list_of_ssubst (cons_ssubst αv ss) := αv::(list_of_ssubst ss).
+
+  Equations ssubst_split {S1 S2} (αs : ssubst (S1++S2)) : ssubst S1 * ssubst S2 :=
+    ssubst_split (S1:=[]) αs := (emp_ssubst,αs);
+    ssubst_split (S1:=u::_) (cons_ssubst αv αs) :=
+      (cons_ssubst αv (ssubst_split αs).1, (ssubst_split αs).2).
+  Lemma interp_scope_ssubst_split {S1 S2} (αs : ssubst (S1++S2)) :
+    interp_scope_split (interp_ssubst αs) ≡
+      (interp_ssubst (ssubst_split αs).1, interp_ssubst (ssubst_split αs).2).
+  Proof.
+    induction S1 as [|u S1]; simpl.
+    - simp ssubst_split. simpl.
+      simp interp_ssubst. done.
+    - dependent elimination αs as [cons_ssubst αv αs].
+      simp ssubst_split. simpl.
+      simp interp_ssubst. repeat f_equiv; eauto; simpl.
+       + rewrite IHS1//.
+       + rewrite IHS1//.
+  Qed.
+
+End interp.
+
+(* Common definitions and lemmas for Kripke logical relations *)
+Section kripke_logrel.
+  Variable s : stuckness.
+
+  Context {sz : nat}.
+  Variable rs : gReifiers sz.
+  Context {R} `{!Cofe R}.
+
+  Notation F := (gReifiers_ops rs).
+  Notation IT := (IT F R).
+  Notation ITV := (ITV F R).
+  Context `{!invGS Σ, !stateG rs R Σ}.
+  Notation iProp := (iProp Σ).
+
+  Context {A:ofe}. (* The type & predicate for the explicit Kripke worlds *)
+  Variable (P : A → iProp).
+  Context `{!NonExpansive P}.
+
+  Implicit Types α β : IT.
+  Implicit Types αv βv : ITV.
+  Implicit Types Φ Ψ : ITV -n> iProp.
+
+  Program Definition expr_pred (α : IT) (Φ : ITV -n> iProp) : iProp :=
+    (∀ x : A, P x -∗ WP@{rs} α @ s {{ v, ∃ y : A, Φ v ∗ P y }}).
+  #[export] Instance expr_pred_ne : NonExpansive2 expr_pred.
+  Proof. solve_proper. Qed.
+  #[export] Instance expr_pred_proper : Proper ((≡) ==> (≡) ==> (≡)) expr_pred .
+  Proof. solve_proper. Qed.
+
+  Definition ssubst_valid {ty} (interp_ty : ty → ITV -n> iProp) {S} (Γ : tyctx ty S) (ss : ssubst S) : iProp :=
+    ([∗ list] τx ∈ zip (list_of_tyctx Γ) (list_of_ssubst (E:=F) ss),
+      interp_ty (τx.1) (τx.2))%I.
+
+  Lemma ssubst_valid_nil {ty} (interp_ty : ty → ITV -n> iProp) :
+    ⊢ ssubst_valid interp_ty empC emp_ssubst.
+  Proof.
+    unfold ssubst_valid.
+    by simp list_of_tyctx list_of_ssubst.
+  Qed.
+
+  Lemma ssubst_valid_cons {ty} (interp_ty : ty → ITV -n> iProp) {S}
+    (Γ : tyctx ty S) (ss : ssubst S) τ αv :
+    ssubst_valid interp_ty (consC τ Γ) (cons_ssubst αv ss)
+    ⊣⊢ interp_ty τ αv ∗ ssubst_valid interp_ty Γ ss.
+  Proof.
+    unfold ssubst_valid.
+    by simp list_of_tyctx list_of_ssubst.
+  Qed.
+
+  Lemma ssubst_valid_app {ty} (interp_ty : ty → ITV -n> iProp)
+    {S1 S2} (Ω1 : tyctx ty S1) (Ω2 : tyctx ty S2) αs :
+    ssubst_valid interp_ty (tyctx_app Ω1 Ω2) αs ⊢
+     ssubst_valid interp_ty Ω1 (ssubst_split αs).1
+   ∗ ssubst_valid interp_ty Ω2 (ssubst_split αs).2.
+  Proof.
+    iInduction Ω1 as [|τ Ω1] "IH" forall (Ω2); simp tyctx_app ssubst_split.
+    - simpl. iIntros "$". iApply ssubst_valid_nil.
+    - iIntros "H".
+      rewrite {4 5}/ssubst_valid.
+      simpl in αs.
+      dependent elimination αs as [cons_ssubst αv αs].
+      simp ssubst_split. simpl.
+      simp list_of_ssubst list_of_tyctx.
+      simpl. iDestruct "H" as "[$ H]".
+      by iApply "IH".
+  Qed.
+
+  Lemma expr_pred_ret α αv Φ `{!IntoVal α αv} :
+    Φ αv ⊢ expr_pred α Φ.
+  Proof.
+    iIntros "H".
+    iIntros (x) "Hx". iApply wp_val.
+    eauto with iFrame.
+  Qed.
+
+  Lemma expr_pred_bind f `{!IT_hom f} α Φ Ψ `{!NonExpansive Φ} :
+    expr_pred α Ψ ⊢
+    (∀ αv, Ψ αv -∗ expr_pred (f (IT_of_V αv)) Φ) -∗
+    expr_pred (f α) Φ.
+  Proof.
+    iIntros "H1 H2".
+    iIntros (x) "Hx".
+    iApply wp_bind.
+    { solve_proper. }
+    iSpecialize ("H1" with "Hx").
+    iApply (wp_wand with "H1").
+    iIntros (βv). iDestruct 1 as (y) "[Hb Hy]".
+    iModIntro.
+    iApply ("H2" with "Hb Hy").
+  Qed.
+
+  Lemma expr_pred_frame α Φ :
+    WP@{rs} α @ s {{ Φ }} ⊢ expr_pred α Φ.
+  Proof.
+    iIntros "H".
+    iIntros (x) "Hx".
+    iApply (wp_wand with "H").
+    eauto with iFrame.
+  Qed.
+End kripke_logrel.
+Arguments expr_pred_bind {_ _ _ _ _ _ _ _ _ _} f {_}.
