vendor/Binding/Core.v
@@ -1,0 +1,295 @@
+Require Import Utf8.
+Require Import RelationClasses Morphisms.
+Require Vector.
+
+Declare Scope bind_scope.
+Delimit Scope bind_scope with bind.
+Local Open Scope bind_scope.
+
+Section EqualityIndexedTypes.
+  Context {Obj : Type}.
+
+  Class EqIndCore (T : Obj → Obj → Type) :=
+    equal A B : T A B → T A B → Prop.
+
+  Class EqInd (T : Obj → Obj → Type) {EIC : EqIndCore T} :=
+    { eq_equiv A B :> Equivalence (equal A B) }.
+
+End EqualityIndexedTypes.
+
+Notation " f ≡ g " := (equal _ _ f%bind g%bind) (at level 70, no associativity) : bind_scope.
+
+(** * Arrows and maps *)
+Section Arrows.
+  Context {Obj : Type}.
+
+  (** ** Arrows *)
+  Class ArrowCore (Arr : Obj → Obj → Type) : Type :=
+    { arrow_id A : Arr A A;
+      arrow_comp {A B C} : Arr B C → Arr A B → Arr A C
+    }.
+
+  Definition arrow {Arr} {ArrEq : EqIndCore Arr} {AC : ArrowCore Arr} := Arr.
+
+  Notation " 'ı' " := (arrow_id _) : bind_scope.
+  Notation " f ∘ g " := (arrow_comp f%bind g%bind) (at level 40, left associativity) : bind_scope.
+
+  Class Arrow (Arr : Obj → Obj → Type) {ArrEq : EqIndCore Arr} {AC : ArrowCore Arr} : Prop :=
+    { arrow_comp_id_l {A B} (f : Arr A B) : ı ∘ f ≡ f;
+      arrow_comp_id_r {A B} (f : Arr A B) : f ∘ ı ≡ f;
+      arrow_comp_assoc {A B C D} (f : Arr C D) (g : Arr B C) (h : Arr A B) :
+        f ∘ g ∘ h ≡ f ∘ (g ∘ h);
+      arrow_comp_proper
+        A B C :> Proper (equal B C ==> equal A B ==> equal A C) arrow_comp}.
+
+  Context {Arr : Obj → Obj → Type} {ArrEq : EqIndCore Arr} {AC : ArrowCore Arr}.
+
+  (** ** Maps *)
+
+  Class FunctorCore (F : Obj → Type) :=
+    fmap : ∀ {A B}, (Arr A B) → F A → F B.
+
+  (*Definition fmap {F : Obj → Type}
+             {FunCore : FunctorCore F} {A B : Obj}
+             (f : Arr A B) : F A → F B := fmap_core _ _ f.*)
+
+  Class Functor (F : Obj → Type) {FunCore : FunctorCore F} : Prop :=
+    { map_id {A} (f : Arr A A) (t : F A) (EQ : f ≡ ı) :
+        fmap f t = t;
+      map_map_comp {A B C} (f : Arr B C) (g : Arr A B) h (t : F A)
+                   (EQ : f ∘ g ≡ h) :
+        fmap f (fmap g t) = fmap h t}.
+
+End Arrows.
+
+(* Repeat notations due to section locality nonsense *)
+Module ArrowNotations.
+  Notation " A '[→]' B " := (arrow A B) (at level 100, no associativity) : type_scope.
+End ArrowNotations.
+  
+Notation " 'ı' " := (arrow_id _) : bind_scope.
+Notation " f ∘ g " := (arrow_comp f%bind g%bind) (at level 40, left associativity) : bind_scope.
+
+(** * Substitutions and binds *)
+Section Substitutions.
+  Context {Obj : Type}.
+
+  (** ** Substitutions *)
+  Class SubstCore (Arr : Obj → Obj → Type) (Sub : Obj → Obj → Type) : Type :=
+    subst_of_arr : ∀ {A B}, Arr A B → Sub A B.
+
+  Definition sub {Arr Sub} {ASC : SubstCore Arr Sub} := Sub.
+  Definition subarr {Arr Sub} {ASC : SubstCore Arr Sub} := Arr.
+
+  (*Notation " 'η' " := (subst_pure _) : bind_scope.
+  Notation " σ • ρ " := (subst_comp σ%bind ρ%bind) (at level 40, left associativity) : bind_scope.*)
+  Notation " f '̂' " := (subst_of_arr f%bind) (at level 30) : bind_scope.
+
+  Class Subst
+        (Arr : Obj → Obj → Type) {ArrEq : EqIndCore Arr} {AC : ArrowCore Arr}
+        (Sub : Obj → Obj → Type) {SubEq : EqIndCore Sub} {SC : ArrowCore Sub}
+        {ASC : SubstCore Arr Sub}  : Prop :=
+    { arrow_subst_id {A} : ı ̂ ≡ (ı : Sub A A);
+      arrow_subst_comp {A B C} (f : Arr B C) (g : Arr A B) :
+        (f ∘ g)̂ ≡ f ̂ ∘ g ̂;
+      arrow_subst_proper A B :> Proper (equal A B ==> equal A B) subst_of_arr}.
+
+    (** ** Binding *)
+
+    Context {Arr : Obj → Obj → Type} {EqArr : EqIndCore Arr} {AC : ArrowCore Arr}.
+    Context {Sub : Obj → Obj → Type} {EqSub : EqIndCore Sub} {SC : ArrowCore Sub}.
+    Context {ASC : SubstCore Arr Sub}.
+
+    Class BindCore (F : Obj → Type) :=
+      bind : ∀ {A B}, (Sub A B) → F A → F B.
+
+    (*Definition bind {F : Obj → Type}
+               {BindF : BindCore F} {A B : Obj}
+               (f : Sub A B) : F A → F B := bind_core _ _ f.*)
+
+    Class BindMapPure (F : Obj → Type) {MapF : FunctorCore F} {BindF : BindCore F} : Prop :=
+      { bind_map {A B} (f : Arr A B) g t
+                 (EQ : f ̂ ≡ g) :
+          fmap f t = bind g t
+      }.
+
+    Class BindMapComm (F : Obj → Type) {MapF : FunctorCore F} {BindF : BindCore F} : Prop :=
+      { bind_map_comm {A B₁ B₂ C} (f₁ : Arr B₁ C) (f₂ : Arr A B₂) (g₁ : Sub A B₁) g₂ t
+                 (EQ : g₂ ∘ f₂ ̂ ≡ f₁ ̂ ∘ g₁) :
+          bind g₂ (fmap f₂ t) = fmap f₁ (bind g₁ t)
+      }.
+
+    Class Bind (F : Obj → Type) {BindF : BindCore F} : Prop :=
+      { bind_pure {A} (f : Sub A A) (t : F A) (EQ : f ≡ ı) :
+          bind f t = t;
+        bind_bind_comp {A B C} (f : Sub B C) (g : Sub A B) h (t : F A)
+                       (EQ : f ∘ g ≡ h) :
+          bind f (bind g t) = bind h t
+      }.
+
+End Substitutions.
+
+Arguments arrow {Obj Arr ArrEq AC} /.
+Arguments sub {Obj Arr Sub ASC } /.
+Arguments subarr {Obj Arr Sub ASC } /.
+
+Module SubNotations.
+  Notation " A '[⇒]' B " := (sub A B) (at level 100, no associativity) : type_scope.
+  Notation " A '[→]' B " := (subarr A B) (at level 100, no associativity) : type_scope.
+End SubNotations.
+Notation " f '̂' " := (subst_of_arr f%bind) (at level 30) : bind_scope.
+
+(** * Lifting *)
+Section Lifting.
+  Context {Obj : Type}.
+
+  Class LiftableCore (Arr : Obj → Obj → Type) (G : Obj → Obj) :=
+    lift : ∀ {A B}, Arr A B → Arr (G A) (G B).
+
+  Notation " f ↑ " := (lift f%bind) (at level 30) : bind_scope.
+
+  Fixpoint liftn {Arr G} {LC : LiftableCore Arr G} {A B : Obj}
+           n (f : Arr A B) : Arr (Nat.iter n G A) (Nat.iter n G B) :=
+    match n with
+    | O => f
+    | S n => (liftn n f) ↑
+    end.
+
+  Class Liftable {Arr} {EqArr : EqIndCore Arr} {AC : ArrowCore Arr}
+        (G : Obj → Obj) {LC : LiftableCore Arr G} : Prop :=
+    { lift_id {A} (f : Arr A A) (EQ : f ≡ ı) : f ↑ ≡ ı;
+      lift_comp {A B C} (f : Arr B C) (g : Arr A B) h (EQ : f ∘ g ≡ h) :
+        f ↑ ∘ g ↑ ≡ h ↑ ;
+      lift_proper A B :> Proper (equal A B ==> equal (G A) (G B)) lift
+    }.
+
+  Context {Arr : Obj → Obj → Type} {EqArr : EqIndCore Arr} {AC : ArrowCore Arr}.
+  Context {Sub : Obj → Obj → Type} {EqSub : EqIndCore Sub} {SC : ArrowCore Sub}.
+  Context {ASC : SubstCore Arr Sub}.
+
+  Class ASLiftInj (G : Obj → Obj) {ALC : LiftableCore Arr G} {SLC : LiftableCore Sub G} : Prop :=
+    lift_of : ∀ {A B} (f : Arr A B) g (EQ : f ̂ ≡ g), f ↑ ̂ ≡ g ↑.
+
+  Class ASLiftComm (G : Obj → Obj)
+        {ALC : LiftableCore Arr G} {SLC : LiftableCore Sub G} : Prop :=
+    lift_comm : ∀ {A B₁ B₂ C} (f₁ : Arr B₁ C) (f₂ : Arr A B₂) (g₁ : Sub A B₁) (g₂ : Sub B₂ C)
+                (EQ : g₂ ∘ f₂ ̂ ≡ f₁ ̂ ∘ g₁),
+      g₂ ↑ ∘ f₂ ↑ ̂ ≡ f₁ ↑ ̂ ∘ g₁ ↑ .
+
+End Lifting.
+
+Arguments Liftable {Obj} Arr {EqArr AC} G {LC}.
+Arguments ASLiftInj {Obj} Arr Sub {EqSub ASC} G {ALC SLC}.
+Arguments ASLiftComm {Obj} Arr Sub {EqSub SC ASC} G {ALC SLC}.
+
+Notation " f ↑ " := (lift f%bind) (at level 30) : bind_scope.
+
+(** * Shifting *)
+Section Shifting.
+  Context {Obj : Type}.
+
+  Class ShiftableCore (Arr : Obj → Obj → Type) (Inc : Obj → Obj) : Type :=
+    mk_shift : ∀ A : Obj, Arr A (Inc A).
+
+  Global Arguments mk_shift {Arr Inc _ A}.
+
+  Definition shift
+             {Arr : Obj → Obj → Type}
+             {F   : Obj → Type} {MapF : FunctorCore F}
+             {Inc : Obj → Obj} {Sh : ShiftableCore Arr Inc}
+             {A : Obj}
+             (a : F A) : F (Inc A) := fmap mk_shift a.
+
+  (*Fixpoint mk_shiftn
+           {Arr : Obj → Obj → Type}
+           {F   : Obj → Type} {map} {MapF : FunctorCore (F:=F) (Arr:=Arr) map}
+           {Inc : Obj → Obj} {AC : ArrowCore Arr} {ALC : ALiftableCore Arr Inc} {Sh : ShiftableCore Arr Inc}
+           {A : Obj} n : Arr A (Nat.iter n Inc A) :=  
+    match n with
+    | O    => ı
+    | S n' => (liftA (G := Inc) (mk_shiftn (Inc := Inc) n')) ∘ mk_shift
+    end.
+
+  Definition shiftn {Arr : Obj → Obj → Type}
+             {F   : Obj → Type} {map} {MapF : FunctorCore (F:=F) (Arr:=Arr) map}
+             {Inc : Obj → Obj} {AC : ArrowCore Arr} {ALC : ALiftableCore Arr Inc} {Sh : ShiftableCore Arr Inc}
+             n {A : Obj} (a : F A) := fmap (mk_shiftn n) a.*)
+
+  Context (Arr : Obj → Obj → Type) {EqArr : EqIndCore Arr} {AC : ArrowCore Arr}.
+  Context (Sub : Obj → Obj → Type) {EqSub : EqIndCore Sub} {SC : ArrowCore Sub}.
+  Context {ASC : SubstCore Arr Sub}.
+  Context (Inc : Obj → Obj) {Sh : ShiftableCore Arr Inc}.
+
+  Class LiftAShift {ALC : LiftableCore Arr Inc} : Prop :=
+    liftA_mk_shift_comm : ∀ {A B : Obj} (f : Arr A B),
+      f ↑ ∘ mk_shift ≡ mk_shift ∘ f.
+
+  Class LiftSShift {SLC : LiftableCore Sub Inc} : Prop :=
+    liftS_mk_shift_comm : ∀ {A B : Obj} (f : Sub A B),
+      f ↑ ∘ mk_shift ̂ ≡ mk_shift ̂ ∘ f.
+
+End Shifting.
+
+Arguments liftA_mk_shift_comm {Obj Arr EqArr AC Inc Sh ALC _ A B} f.
+Arguments liftS_mk_shift_comm {Obj Arr Sub EqSub SC ASC Inc  Sh SLC _ A B} f.
+
+(** * Substituting *)
+Section Substituting.
+  Context {Obj : Type}.
+
+  Class SubstitutableCore
+        (Sub : Obj → Obj → Type) (F : Obj → Type) (Inc : Obj → Obj) : Type :=
+    mk_subst : ∀ {A : Obj} (x : F A), Sub (Inc A) A.
+
+  Definition subst
+             {Sub : Obj → Obj → Type}
+             {G   : Obj → Type} {BindG : BindCore G}
+             {F   : Obj → Type} {Inc : Obj → Obj} {Sb : SubstitutableCore Sub F Inc}
+             {A : Obj}
+             (a : G (Inc A)) (v : F A) : G A := bind (mk_subst v) a.
+
+  (*
+  Fixpoint mk_substV
+           {Sub : Obj → Obj → Type} {Arr : Obj → Obj → Type}
+           {G   : Obj → Type} {bnd} {BindG : BindCore (F:=G) (Sub:=Sub) bnd}
+           {F   : Obj → Type} {Inc : Obj → Obj} {PSC : PreSubstCore Sub} {AC : ArrowCore Arr}
+           {SC : SubstCore Arr Sub} {SLC : SLiftableCore Sub Inc} {Sb : SubstitutableCore Sub F Inc}
+           {A : Obj} {n} (xs : Vector.t (F A) n) : Sub (Nat.iter n Inc A) A :=
+    match xs with
+    | Vector.nil _         => η
+    | Vector.cons _ x _ xs => (mk_subst (Inc := Inc) x) • (mk_substV (Inc := Inc) xs) ⇑
+    end.
+
+  Definition substV
+             {Sub : Obj → Obj → Type} {Arr : Obj → Obj → Type} {AC : ArrowCore Arr}
+             {G   : Obj → Type} {bnd} {BindG : BindCore (F:=G) (Sub:=Sub) bnd}
+             {F   : Obj → Type} {Inc : Obj → Obj} {PSC : PreSubstCore Sub} {SC : SubstCore Arr Sub}
+             {SLC : SLiftableCore Sub Inc} {Sb : SubstitutableCore Sub F Inc}
+             {A : Obj} {n} (xs : Vector.t (F A) n) (a : G (Nat.iter n Inc A)) : G A :=
+    bind (mk_substV xs) a.
+   *)
+  
+  Context (Arr : Obj → Obj → Type) {EqArr : EqIndCore Arr} {AC : ArrowCore Arr}.
+  Context (Sub : Obj → Obj → Type) {EqSub : EqIndCore Sub} {SC : ArrowCore Sub}.
+  Context {ASC : SubstCore Arr Sub}.
+  Context (F : Obj → Type) (Inc : Obj → Obj) {Sb : SubstitutableCore Sub F Inc}.
+
+  Class SubstShift {Sh : ShiftableCore Arr Inc} : Prop :=
+    subst_shift_pure : ∀ {A : Obj} (v : F A),
+      mk_subst v ∘ mk_shift ̂ ≡ ı.
+
+  Class SubstFMap {MapF : FunctorCore F}
+        {ALC : LiftableCore Arr Inc} : Prop :=
+    map_mk_subst_comm : ∀ {A B : Obj} (f : Arr A B) (v : F A),
+      f ̂ ∘ mk_subst v ≡ mk_subst (fmap f v) ∘ f ↑ ̂.
+
+  Class SubstBind {BndF : BindCore F}
+        {SLC : LiftableCore Sub Inc} : Prop :=
+    bind_mk_subst_comm : ∀ {A B : Obj} (f : Sub A B) (v : F A),
+      f ∘ mk_subst v ≡ mk_subst (bind f v) ∘ f ↑.
+
+End Substituting.
+
+Arguments subst_shift_pure {Obj Arr Sub EqSub SC ASC F Inc Sb Sh _ A} v.
+Arguments map_mk_subst_comm {Obj Arr Sub EqSub SC ASC F Inc Sb MapF ALC _ A B} f v.
+Arguments bind_mk_subst_comm {Obj Sub EqSub SC F Inc Sb BndF SLC _ A B} f v.
