vendor/Binding/Inc.v
@@ -1,0 +1,25 @@
+Require Import Utf8.
+
+Notation "∅" := Empty_set.
+
+Inductive inc (V : Set) : Set :=
+| VZ : inc V
+| VS : V → inc V
+.
+
+Arguments VZ {V}.
+Arguments VS {V}.
+
+Definition inc_map {A B : Set} (f : A → B) (m : inc A) : inc B :=
+  match m with
+  | VZ   => VZ
+  | VS x => VS (f x)
+  end.
+
+Fixpoint nth_inc n {A : Set} : Nat.iter n inc (inc A) :=
+  match n with
+  | O   => VZ
+  | S n => VS (nth_inc n)
+  end.
+
+Notation "& n" := (nth_inc n) (at level 5).
