vendor/Binding/Intrinsic.v
@@ -1,0 +1,232 @@
+Require Import Utf8.
+Require Import Binding.Core.
+Require Import Binding.Inc.
+Require Import Binding.Properties.
+Require Import Morphisms.
+
+Record Ctx {V : Type} :=
+  {dom : Set;
+   arr :> dom -> V
+  }.
+Arguments Ctx V : clear implicits.
+
+Definition mtC {V : Type} : Ctx V :=
+  {| dom := Empty_set;
+     arr x := match x with end
+  |}.
+
+Definition extC {V : Type} (v : V) (Γ : Ctx V) : Ctx V :=
+  {| dom := inc (dom Γ);
+     arr x := match x with
+              | VZ => v
+              | VS x => Γ x
+              end
+  |}.
+
+Notation "'ε'" := mtC.
+Notation "Γ ▹ v" := (extC v Γ) (at level 40, left associativity).
+
+Class IntPureCore {V : Type} (F : V → Ctx V → Type) : Type :=
+  int_pure : ∀ (Γ : Ctx V) v (x : dom Γ) (EQ : Γ x = v) , F v Γ.
+
+Arguments int_pure {V F _ Γ}.
+
+Record Arr {V : Type} {Γ Δ : Ctx V} : Type :=
+  { apply_arr : dom Γ → dom Δ;
+    arr_hom   : ∀ x : dom Γ, Δ (apply_arr x) = Γ x
+  }.
+Arguments Arr {V} Γ Δ.
+Notation " A '[→]' B " := (Arr A B) (at level 100, no associativity) : type_scope.
+Coercion apply_arr : Arr >-> Funclass.
+
+Record Sub {V} {F : V → Ctx V → Type} {FP : IntPureCore F} (Γ Δ : Ctx V) : Type :=
+  { apply_sub : ∀ v (x : dom Γ) (EQ : Γ x = v), F v Δ
+  }.
+Notation " A '[⇒]' B " := (Sub A B) (at level 100, no associativity) : type_scope.
+
+Arguments apply_sub {V F FP Γ Δ}.
+Coercion apply_sub : Sub >-> Funclass.
+
+Global Instance ArrEqC {V} : EqIndCore (Arr (V := V)) :=
+  λ A B f g, ∀ x, f x = g x.
+
+Global Instance ArrEq {V} : EqInd (Arr (V := V)).
+Proof.
+  split; intros; split; intros; congruence.
+Qed.
+
+Global Instance SubEqC {V F} {FP : IntPureCore (V := V) F} : EqIndCore Sub :=
+  λ A B f g, ∀ v x EQ, f v x EQ = g v x EQ.
+
+Global Instance SubEq {V F} {FP : IntPureCore (V := V) F} : EqInd Sub.
+Proof.
+  split; split; intros; congruence.
+Qed.
+
+Global Program Instance ArrowCore_Set {V} : ArrowCore (Arr (V := V)) :=
+  { arrow_id   := λ _,         {| apply_arr := λ x, x       |}
+  ; arrow_comp := λ _ _ _ f g, {| apply_arr := λ x, f (g x) |}
+  }.
+Next Obligation.
+  etransitivity; apply arr_hom.
+Defined.
+
+Class IntPure {V} (F : V → Ctx V → Type) {FP : IntPureCore (V := V) F}
+    {MapF : ∀ v, FunctorCore (F v)}
+    {BndF : ∀ v, BindCore (Sub := Sub) (F v)} : Prop :=
+  { fmap_int_pure : ∀ (Γ Δ : Ctx V) (f : Arr Γ Δ) v (x : dom Γ) (EQ : Γ x = v),
+        fmap f (int_pure v x EQ) = int_pure v (f x) (eq_trans (arr_hom f x) EQ)
+  ; bind_set_pure : ∀ (Γ Δ : Ctx V) (f : Sub Γ Δ) v (x : dom Γ) (EQ : Γ x = v),
+      bind f (int_pure (IntPureCore := FP) v x EQ) = f v x EQ
+  }.
+
+Section IntInstances.
+  Context {V} {F : V → Ctx V → Type} {FP : IntPureCore F}.
+  Context {MapF : ∀ v, FunctorCore (Arr := Arr) (F v)}.
+  Context {BndF : ∀ v, BindCore (Sub := Sub) (F v)}.
+  Context {SPF : IntPure F}.
+
+  Global Instance Arrow_Int : Arrow (Arr (V := V)).
+  Proof.
+    split; [unfold equal, ArrEqC; simpl; congruence .. |].
+    intros A B C f₁ f₂ EQf g₁ g₂ EQg x; simpl; congruence.
+  Qed.
+
+  Global Instance SubstArrCore_Set : ArrowCore (Sub (V := V)) :=
+    { arrow_id A := {| apply_sub := int_pure |};
+      arrow_comp A B C f g := {| apply_sub := λ v x EQ, bind f (g v x EQ) |} }.
+
+  Global Instance SubstCore_Set : SubstCore Arr Sub :=
+    λ Γ Δ f, {| apply_sub := λ v x EQ, int_pure v (f x) (eq_trans (arr_hom f x) EQ) |}.
+
+  Program Definition extFun v (Γ Δ : Ctx V) (f : Arr Γ Δ) : Arr (Γ ▹ v) (Δ ▹ v) :=
+    {| apply_arr := inc_map f |}.
+  Next Obligation.
+    destruct x as [| x]; simpl; [reflexivity | apply arr_hom].
+  Defined.
+
+  Context {MF : ∀ v, Functor (F v)} {BF : ∀ v, Bind (F v)}.
+  Context {BMPF : ∀ v, BindMapPure (F v)} {BMCF : ∀ v, BindMapComm (F v)}.
+
+  Global Instance SubArrow_Set : Arrow Sub.
+  Proof.
+    split; simpl; intros.
+    - intros v x EQ; simpl; apply bind_pure; reflexivity.
+    - intros v x EQ; simpl; apply bind_set_pure.
+    - intros v x EQ; simpl; symmetry; apply bind_bind_comp; reflexivity.
+    - intros ρ₁ ρ₂ EQρ σ₁ σ₂ EQσ v x EQ; simpl; rewrite EQσ; clear EQσ.
+      etransitivity; [| apply bind_pure; reflexivity].
+      symmetry; apply bind_bind_comp.
+      intros u y EQ'; rewrite EQρ; apply bind_pure; reflexivity.
+  Qed.
+
+  Global Instance Subst_Set : Subst Arr Sub.
+  Proof.
+    split; intros.
+    - intros v x []; simpl; reflexivity.
+    - intros v x []; simpl; symmetry; unfold ArrowCore_Set_obligation_2.
+      generalize (g x) as y, (arr_hom g x).
+      intros y []; simpl; apply bind_set_pure.
+    - intros f g EQ v x EQ'; simpl.
+      rewrite <- !fmap_int_pure, EQ; reflexivity.
+  Qed.
+
+  Global Instance ALiftableCore_ext {v : V} : LiftableCore Arr (extC v) :=
+    { lift := extFun v }.
+
+  Global Instance ALiftable_ext {v : V} : Liftable Arr (extC v).
+  Proof.
+    split; intros.
+    - intros [| x]; simpl; [reflexivity | f_equal; apply EQ].
+    - intros [| x]; simpl; [reflexivity | f_equal; apply EQ].
+    - intros f₁ f₂ EQf [| x]; simpl; [reflexivity | f_equal; apply EQf].
+  Qed.
+
+  Global Program Instance ShiftableCore_ext {v : V} : ShiftableCore Arr (extC v) :=
+    λ A, {| apply_arr := VS : dom A → dom (A ▹ v) |}.
+
+  Global Instance LiftAShift_ext {v : V} : LiftAShift Arr (extC v).
+  Proof.
+    unfold LiftAShift; intros Γ Δ f x; reflexivity.
+  Qed.
+
+  Global Instance SLiftableCore_ext {v : V} : LiftableCore Sub (extC v) :=
+    { lift Γ Δ ρ :=
+        {| apply_sub := λ u (x : dom (Γ ▹ v)),
+                        match x with
+                        | VZ   => λ EQ, int_pure u (VZ : dom (Δ ▹ v)) EQ
+                        | VS y => λ EQ, shift (ρ u y EQ)
+                        end
+        |}
+    }.
+
+  Global Instance LiftSShift_ext {v : V} : LiftSShift Arr Sub (extC v).
+  Proof.
+    intros A B f u x []; simpl.
+    rewrite bind_set_pure.
+    apply map_to_bind.
+  Qed.
+
+  Global Instance SLiftable_ext {v : V} : Liftable Sub (extC v).
+  Proof.
+    split; intros.
+    - intros u [| x] []; simpl; [reflexivity | unfold shift; simpl].
+      rewrite EQ; simpl.
+      rewrite fmap_int_pure; simpl; reflexivity.
+    - intros u [| x] []; simpl; [now apply bind_set_pure |].
+      rewrite bind_liftS_shift_comm, <- EQ; reflexivity.
+    - intros f₁ f₂ EQf u [| x] []; simpl; [reflexivity | now rewrite EQf].
+  Qed.
+
+  Global Instance ASLiftInj_ext {v : V} : ASLiftInj Arr Sub (extC v).
+  Proof.
+    intros A B f g EQ u [| x] []; simpl; [reflexivity |].
+    rewrite <- EQ; simpl; symmetry.
+    generalize (f x) as y, (arr_hom f x); intros y []; simpl.
+    unfold shift; rewrite fmap_int_pure; reflexivity.
+  Qed.
+
+  Global Instance ASLiftComm_ext {v : V} : ASLiftComm Arr Sub (extC v).
+  Proof.
+    intros A B₁ B₂ C f₁ f₂ g₁ g₂ EQ u [| x] []; simpl.
+    - etransitivity; [apply bind_set_pure |].
+      rewrite bind_set_pure; reflexivity.
+    - unfold shift; erewrite <- map_to_bind, map_map_comp by apply liftA_mk_shift_comm.
+      rewrite <- map_map_comp'; specialize (EQ _ x eq_refl); simpl in EQ; rewrite <- map_to_bind in EQ.
+      rewrite <- EQ; clear EQ.
+      generalize (f₂ x) as y, (arr_hom f₂ x); intros y []; simpl.
+      rewrite !bind_set_pure; reflexivity.
+  Qed.
+
+  Global Instance SubstitutableCore_ext {v : V} : SubstitutableCore Sub (F v) (extC v) :=
+    λ A u,
+    {| apply_sub := λ w (x : dom (A ▹ v)),
+                    match x with
+                    | VZ => λ EQ, match EQ with eq_refl => u end
+                    | VS y => int_pure w y
+                    end
+    |}.
+
+  Global Instance SubstShift_ext {v : V} : SubstShift Arr Sub (F v) (extC v).
+  Proof.
+    intros A u w x []; simpl.
+    apply bind_set_pure.
+  Qed.
+
+  Global Instance SubstFMap_ext {v : V} : SubstFMap Arr Sub (F v) (extC v).
+  Proof.
+    intros A B f u w [ | x ] []; simpl.
+    - rewrite <- map_to_bind, bind_set_pure; simpl; reflexivity.
+    - rewrite !bind_set_pure; simpl; reflexivity.
+  Qed.
+
+  Global Instance SubstBind_ext {v : V} : SubstBind Sub (F v) (extC v).
+  Proof.
+    intros A B f u w [| x] []; simpl.
+    - rewrite bind_set_pure; reflexivity.
+    - rewrite bind_set_pure; symmetry; apply subst_shift_id.
+  Qed.
+
+End IntInstances.
+
+Arguments int_pure {V F _ Γ v} /.
