vendor/Binding/Lib.v
@@ -1,0 +1,4 @@
+Require Export Binding.Core.
+Require Export Binding.Inc.
+Require Export Binding.Properties.
+Require Export Binding.TermSimpl.
