vendor/Binding/Product.v
@@ -1,0 +1,130 @@
+Require Import Utf8.
+Require Import Binding.Lib.
+
+Record sprod (U₁ U₂ : Type) : Type :=
+  { π₁ : U₁
+  ; π₂ : U₂
+  }.
+
+Arguments π₁ {U₁ U₂}.
+Arguments π₂ {U₁ U₂}.
+
+Notation "U₁ × U₂" := (sprod U₁ U₂) (at level 40) : type_scope.
+Notation "⟨ A , B ⟩" := {| π₁ := A ; π₂ := B |} : bind_scope.
+
+Section Defs.
+  Context {U₁ U₂ : Type} {Arr₁ : U₁ → U₁ → Type} {Arr₂ : U₂ → U₂ → Type}
+          {EA₁ : EqIndCore Arr₁} {EA₂ : EqIndCore Arr₂} {EqA₁ : EqInd Arr₁} {EqA₂ : EqInd Arr₂}
+          {AC₁ : ArrowCore Arr₁} {AC₂ : ArrowCore Arr₂} {AR₁ : Arrow Arr₁} {AR₂ : Arrow Arr₂}.
+
+  Local Open Scope bind_scope.
+  Import ArrowNotations.
+
+  Record prod_arr {X Y : U₁ × U₂} : Type :=
+    { arr₁ : Arr₁ (π₁ X) (π₁ Y);
+      arr₂ : Arr₂ (π₂ X) (π₂ Y)
+    }.
+  Global Arguments prod_arr X Y : clear implicits.
+
+  Notation " f × g " := {| arr₁ := f ; arr₂ := g |} (at level 40) : bind_scope.
+
+  Global Instance EIC_prod : EqIndCore prod_arr :=
+    λ A B f g, arr₁ f ≡ arr₁ g ∧ arr₂ f ≡ arr₂ g.
+
+  Global Instance ArrowCore_vsig_arr : ArrowCore prod_arr :=
+    {| arrow_id A := ı × ı;
+       arrow_comp A B C f g := (arr₁ f ∘ arr₁ g) × (arr₂ f ∘ arr₂ g) |}.
+
+  Global Instance Eq_prod : EqInd prod_arr.
+  Proof.
+    split; split; intros.
+    - split; reflexivity.
+    - split; symmetry; apply H.
+    - split; etransitivity; now (apply H || apply H0).
+  Qed.
+
+  Global Instance Arrow_prod_arr : Arrow prod_arr.
+  Proof.
+    split; intros.
+    - split; apply arrow_comp_id_l.
+    - split; apply arrow_comp_id_r.
+    - split; apply arrow_comp_assoc.
+    - split; eapply arrow_comp_proper; now (apply H0 || apply H).
+  Qed.
+
+  Definition at₁ {A B : U₁} {C : U₂} (f : A [→] B) : ⟨A, C⟩ [→] ⟨B, C⟩ :=
+    (f : π₁ ⟨A, C⟩ [→] π₁ ⟨B, C⟩) × ı.
+  Definition at₂ {A : U₁} {B C : U₂} (f : B [→] C) : ⟨A, B⟩ [→] ⟨A, C⟩ :=
+    ı × (f : π₂ ⟨A, B⟩ [→] π₂ ⟨A, C⟩).
+
+  Section ALift.
+    Context (F₁ : U₁ → U₁) (F₂ : U₂ → U₂) {ALC₁ : LiftableCore Arr₁ F₁}
+            {ALC₂ : LiftableCore Arr₂ F₂} {AL₁ : Liftable Arr₁ F₁} {AL₂ : Liftable Arr₂ F₂}.
+
+    Definition on₁ (X : U₁ × U₂) := ⟨ F₁ (π₁ X), π₂ X ⟩.
+    Definition on₂ (X : U₁ × U₂) := ⟨ π₁ X, F₂ (π₂ X) ⟩.
+
+    Global Instance ALC_prod_left : LiftableCore prod_arr on₁ :=
+      { lift A B f := (arr₁ f) ↑ × (arr₂ f : π₂ (on₁ A) [→] π₂ (on₁ B))}.
+
+    Global Instance AL_prod_left : Liftable prod_arr on₁.
+    Proof.
+      split; intros.
+      - split; simpl; [apply lift_id |]; apply EQ.
+      - split; simpl; [apply lift_comp |]; apply EQ.
+      - split; simpl; [apply lift_proper |]; apply H.
+    Qed.
+
+    Global Instance ALC_prod_right : LiftableCore prod_arr on₂ :=
+      { lift A B f := (arr₁ f : π₁ (on₂ A) [→] π₁ (on₂ B)) × (arr₂ f) ↑}.
+
+    Global Instance AL_prod_right : Liftable prod_arr on₂.
+    Proof.
+      split; intros.
+      - split; simpl; [| apply lift_id]; apply EQ.
+      - split; simpl; [| apply lift_comp]; apply EQ.
+      - split; simpl; [| apply lift_proper]; apply H.
+    Qed.
+
+  End ALift.
+
+  Section Shift.
+    Context (Inc₁ : U₁ → U₁) (Inc₂ : U₂ → U₂)
+            {SC₁ : ShiftableCore Arr₁ Inc₁} {SC₂ : ShiftableCore Arr₂ Inc₂}.
+
+    Global Instance SC_prod_left : ShiftableCore prod_arr (on₁ Inc₁) :=
+      { mk_shift := λ A, mk_shift × ı }.
+
+    Global Instance SC_prod_right : ShiftableCore prod_arr (on₂ Inc₂) :=
+      { mk_shift := λ A, ı × mk_shift }.
+
+  End Shift.
+
+  Section LiftA_Shift.
+    Context (F₁ : U₁ → U₁) (F₂ : U₂ → U₂)
+            {ALC₁ : LiftableCore Arr₁ F₁} {ALC₂ : LiftableCore Arr₂ F₂}
+            {AL₁ : Liftable Arr₁ F₁} {AL₂ : Liftable Arr₂ F₂}
+            {SC₁ : ShiftableCore Arr₁ F₁} {SC₂ : ShiftableCore Arr₂ F₂}
+            {LAS₁ : LiftAShift Arr₁ F₁} {LAS₂ : LiftAShift Arr₂ F₂}.
+
+    Global Instance LiftAShift_prod_left : LiftAShift prod_arr (on₁ F₁).
+    Proof.
+      intros A B f; split; simpl.
+      - apply LAS₁.
+      - etransitivity; [ apply arrow_comp_id_r | ].
+        symmetry; apply arrow_comp_id_l.
+    Qed.
+
+
+    Global Instance LiftAShift_prod_right : LiftAShift prod_arr (on₂ F₂).
+    Proof.
+      intros A B f; split; simpl.
+      - etransitivity; [ apply arrow_comp_id_r | ].
+        symmetry; apply arrow_comp_id_l.
+      - apply LAS₂.
+    Qed.
+  End LiftA_Shift.
+
+End Defs.
+
+Notation " f × g " := {| arr₁ := f ; arr₂ := g |} (at level 40) : bind_scope.
